nat.lean
@@ -1,7 +1,10 @@
 import ground_zero.equiv ground_zero.coproduct
+import ground_zero.support
 open ground_zero
 
 namespace ground_zero.nat
+
+universes u v w
 
 def code : ℕ → ℕ + unit
 | nat.zero := coproduct.inr unit.star
@@ -19,6 +22,37 @@ theorem closed_nat : ℕ ≃ ℕ + unit := begin
   { intro n, simp, induction n,
     { simp [decode, code] },
     { induction n, simp [code, decode] } }
+end
+
+theorem equiv_addition (α : Type u) (β : Type v) (γ : Type w)
+  (e : α ≃ β) : α + γ ≃ β + γ := begin
+  induction e with f H,
+  have q := qinv.b2q f H,
+  cases q with g inv, cases inv with α' β',
+
+  simp [equiv.homotopy, function.comp] at α',
+  simp [equiv.homotopy, function.comp] at β',
+
+  let f : α + γ → β + γ := λ x, match x with
+  | coproduct.inl a := coproduct.inl (f a)
+  | coproduct.inr c := coproduct.inr c
+  end,
+  let g : β + γ → α + γ := λ x, match x with
+  | coproduct.inl b := coproduct.inl (g b)
+  | coproduct.inr c := coproduct.inr c
+  end,
+
+  existsi f, split; existsi g,
+  { intro x, induction x,
+    { simp [g, f],
+      rw [support.to_builtin (β' x)],
+      simp },
+    { trivial } },
+  { intro x, induction x,
+    { simp [f, g],
+      rw [support.to_builtin (α' x)],
+      simp },
+    { trivial } }
 end
 
 end ground_zero.nat
